Fix ILN for external events.

IL/ILN.v
@@ -1,5 +1,5 @@
 Require Import List.
-Require Export Util Var Val Exp Env Map CSet AutoIndTac IL Sim Infra.Status.
+Require Export Util Var Val Exp Env Map CSet AutoIndTac IL Bisim Infra.Status.
 
 Set Implicit Arguments.
 
@@ -8,14 +8,15 @@ Open Scope map_scope.
 Inductive nstmt : Type :=
 | nstmtExp    (x : var) (e: exp) (s : nstmt)
 | nstmtIf     (e : exp) (s : nstmt) (t : nstmt)
-| nstmtGoto   (l : lab) (Y:args) 
-| nstmtReturn (e : exp) 
-(* block f Z : rt = s in b *)    
+| nstmtGoto   (l : lab) (Y:args)
+| nstmtReturn (e : exp)
+| nstmtExtern (x : var) (f:external) (Y:args) (s:nstmt)
+(* block f Z : rt = s in b *)
 | nstmtLet    (l : lab) (Z:params) (s : nstmt) (t : nstmt).
 
 
 Fixpoint pos X `{OrderedType X} (l:list X) (x:X) (n:nat) : option nat :=
-  match l with 
+  match l with
     | nil => None
     | y::l => if [ x === y ] then Some n else pos l x (S n)
   end.
@@ -30,66 +31,76 @@ Module F.
         block_E : onv val;
         block_F : lab * params * nstmt
       }.
-  
+
   Definition labenv := onv block.
   Definition state : Type := (labenv * onv val * nstmt)%type.
 
-  Inductive step : state -> state -> Prop :=
+  Inductive step : state -> event -> state -> Prop :=
   | nstepExp L E x e b v
     (def:exp_eval E e = Some v)
-    : step (L, E, nstmtExp x e b) (L, E[x<-Some v], b)
+    : step (L, E, nstmtExp x e b) EvtTau (L, E[x<-Some v], b)
 
   | nstepIfT L E
     (e:exp) b1 b2 v
     (def:exp_eval E e = Some v)
     (condTrue: val2bool v = true)
-    : step (L, E, nstmtIf e b1 b2) (L, E, b1)
-    
+    : step (L, E, nstmtIf e b1 b2) EvtTau (L, E, b1)
+
   | nstepIfF L E
     (e:exp) b1 b2 v
     (def:exp_eval E e = Some v)
     (condFalse:val2bool v = false)
-    : step (L, E, nstmtIf e b1 b2) (L, E, b2)
+    : step (L, E, nstmtIf e b1 b2) EvtTau (L, E, b2)
 
-    
+
   | nstepGoto (L:labenv) (E:onv val) (l l':lab) Y Z (s:nstmt) L' E'
     (len:length Z = length Y)
-    (lEQ:l = l') (* hack: otherwise inversions confuse guardedness checker in 
+    (lEQ:l = l') (* hack: otherwise inversions confuse guardedness checker in
                   simulation proofs*)
-    
+
     (Ldef:L (counted l) = Some (blockI L' E' (l',Z,s))) E'' vl
     (def:omap (exp_eval E) Y = Some vl)
     (updOk:E'[Z <-- List.map Some vl]  = E'')
     : step (L, E, nstmtGoto l Y)
+           EvtTau
            (L'[(counted l) <- Some (blockI L' E' (l,Z,s))], E'', s)
 
-  | stepLet L E f s Z t 
-    : step (L, E, nstmtLet f Z s t) (L[counted f <- Some (blockI L E (f,Z,s))], E, t).
+  | stepLet L E f s Z t
+    : step (L, E, nstmtLet f Z s t) EvtTau (L[counted f <- Some (blockI L E (f,Z,s))], E, t)
 
-  Lemma step_functional :
-    functional step.
+  | stepExtern L E x f Y s vl v
+    (def:omap (exp_eval E) Y = Some vl)
+    : step  (L, E, nstmtExtern x f Y s)
+            (EvtExtern (ExternI f vl v))
+            (L, E[x <- Some v], s).
+
+
+  Lemma step_internally_deterministic :
+    internally_deterministic step.
   Proof.
-    induction 1; inversion 1; intros; subst; repeat get_functional; try congruence. 
+    hnf; intros. inv H; inv H0; split; eauto; try congruence.
   Qed.
 
-  Lemma step_dec 
+  Lemma step_dec
   : reddec step.
   Proof.
     hnf; intros. destruct x as [[L V] []].
-    - case_eq (exp_eval V e); intros. left. eauto using step.
+    - case_eq (exp_eval V e); intros. left. eexists EvtTau; eauto using step.
       right. stuck.
-    - case_eq (exp_eval V e); intros. 
-      left. case_eq (val2bool v); intros; eauto using step.
+    - case_eq (exp_eval V e); intros.
+      left. case_eq (val2bool v); intros; eexists EvtTau; eauto using step.
       right. stuck.
-    - case_eq (L (counted l)); intros. 
+    - case_eq (L (counted l)); intros.
       + destruct b as [? ? [[? ?] ?]].
         decide (l = l0); subst; try now (right; stuck).
         decide (length l1 = length Y); try now (right; stuck).
         case_eq (omap (exp_eval V) Y); intros; try now (right; stuck).
-        left. econstructor. econstructor; eauto.
-      + right. stuck. 
+        left. eexists EvtTau. econstructor. econstructor; eauto.
+      + right. stuck.
     - right. stuck.
-    - left. eauto using step.
+    - case_eq (omap (exp_eval V) Y); intros; try now (right; stuck).
+      left. eexists (EvtExtern (ExternI f l 0)). eauto using step.
+    - left. exists EvtTau. eauto using step.
   Qed.
 
 End F.
@@ -103,27 +114,27 @@ Module I.
         block_L : onv block;
         block_F : lab * params * nstmt
       }.
-  
+
   Definition labenv := onv block.
   Definition state : Type := (labenv * onv val * nstmt)%type.
   Definition labenv_empty : labenv := fun _ => None.
 
-  Inductive step : state -> state -> Prop :=
+  Inductive step : state -> event -> state -> Prop :=
   | nstepExp L E x e b v
     (def:exp_eval E e = Some v)
-    : step (L, E, nstmtExp x e b) (L, E[x<-Some v], b)
+    : step (L, E, nstmtExp x e b) EvtTau (L, E[x<-Some v], b)
 
   | nstepIfT L E
     (e:exp) b1 b2 v
     (def:exp_eval E e = Some v)
     (condTrue: val2bool v = true)
-    : step (L, E, nstmtIf e b1 b2) (L, E, b1)
-    
+    : step (L, E, nstmtIf e b1 b2) EvtTau (L, E, b1)
+
   | nstepIfF L E
     (e:exp) b1 b2 v
     (def:exp_eval E e = Some v)
     (condFalse:val2bool v = false)
-    : step (L, E, nstmtIf e b1 b2) (L, E, b2)
+    : step (L, E, nstmtIf e b1 b2) EvtTau (L, E, b2)
 
   | nstepGoto (L:labenv) (E:onv val) (l l':lab) Y Z (s:nstmt) L' vl
     (len:length Z = length Y)
@@ -132,36 +143,47 @@ Module I.
     (def:omap (exp_eval E) Y = Some vl)
     (updOk:E [Z <-- List.map Some vl]  = E'')
     : step (L, E, nstmtGoto l Y)
+           EvtTau
            (L'[(counted l) <- Some (blockI L' (l,Z,s))], E'', s)
 
-  | stepLet L E f s Z t 
-    : step (L, E, nstmtLet f Z s t) (L[counted f <- Some (blockI L (f,Z,s))], E, t).
+  | stepLet L E f s Z t
+    : step (L, E, nstmtLet f Z s t)
+           EvtTau
+           (L[counted f <- Some (blockI L (f,Z,s))], E, t)
 
-  Lemma step_functional :
-    functional step.
+  | stepExtern L E x f Y s vl v
+    (def:omap (exp_eval E) Y = Some vl)
+    : step  (L, E, nstmtExtern x f Y s)
+            (EvtExtern (ExternI f vl v))
+            (L, E[x <- Some v], s).
+
+
+  Lemma step_internally_deterministic :
+    internally_deterministic step.
   Proof.
-    induction 1; inversion 1; intros; subst; repeat get_functional; try congruence. 
+    hnf; intros. inv H; inv H0; split; eauto; try congruence.
   Qed.
 
-
-  Lemma step_dec 
+  Lemma step_dec
   : reddec step.
   Proof.
     hnf; intros. destruct x as [[L V] []].
-    - case_eq (exp_eval V e); intros. left. eauto using step.
+    - case_eq (exp_eval V e); intros. left. eexists EvtTau; eauto using step.
       right. stuck.
-    - case_eq (exp_eval V e); intros. 
-      left. case_eq (val2bool v); intros; eauto using step.
+    - case_eq (exp_eval V e); intros.
+      left. case_eq (val2bool v); intros; eexists EvtTau; eauto using step.
       right. stuck.
-    - case_eq (L (counted l)); intros. 
-      + destruct b as [ ? [[? ?] ?]].
+    - case_eq (L (counted l)); intros.
+      + destruct b as [? [[? ?] ?]].
         decide (l = l0); subst; try now (right; stuck).
         decide (length l1 = length Y); try now (right; stuck).
         case_eq (omap (exp_eval V) Y); intros; try now (right; stuck).
-        left. econstructor. econstructor; eauto.
-      + right. stuck. 
+        left. eexists EvtTau. econstructor. econstructor; eauto.
+      + right. stuck.
     - right. stuck.
-    - left. eauto using step.
+    - case_eq (omap (exp_eval V) Y); intros; try now (right; stuck).
+      left. eexists (EvtExtern (ExternI f l 0)). eauto using step.
+    - left. exists EvtTau. eauto using step.
   Qed.
 
 End I.
@@ -169,14 +191,16 @@ End I.
 Fixpoint labIndices (s:nstmt) (symb: list lab) : status stmt :=
   match s with
     | nstmtExp x e s => sdo s' <- (labIndices s symb); Success (stmtExp x e s')
-    | nstmtIf x s1 s2 => 
+    | nstmtIf x s1 s2 =>
       sdo s1' <- (labIndices s1 symb);
       sdo s2' <- (labIndices s2 symb);
       Success (stmtIf x s1' s2')
-    | nstmtGoto l Y => 
+    | nstmtGoto l Y =>
       sdo f <- option2status (pos symb l 0) "labIndices: Undeclared function" ; Success (stmtGoto (LabI f) Y)
     | nstmtReturn x => Success (stmtReturn x)
-    | nstmtLet l Z s1 s2 => 
+    | nstmtExtern x f Y s =>
+      sdo s' <- (labIndices s symb); Success (stmtExtern x f Y s')
+    | nstmtLet l Z s1 s2 =>
       sdo s1' <- labIndices s1 (l::symb);
       sdo s2' <- labIndices s2 (l::symb);
       Success (stmtLet Z s1' s2')
@@ -191,11 +215,11 @@ Definition state_result X (s:X*onv val*nstmt) : option val :=
 Instance statetype_I : StateType I.state := {
   step := I.step;
   result := (@state_result I.labenv);
-  step_dec := I.step_dec; 
-  step_functional := I.step_functional
-}. 
+  step_dec := I.step_dec;
+  step_internally_deterministic := I.step_internally_deterministic
+}.
 
-Tactic Notation "goto_invs" tactic(tac) :=
+(*Tactic Notation "goto_invs" tactic(tac) :=
   match goal with
     | [ |- sim (?L, _, nstmtGoto ?l ?Y) (_, _, _) ] =>
       let b := fresh "blk" in
@@ -206,18 +230,18 @@ Tactic Notation "goto_invs" tactic(tac) :=
                   [ tac | no_step ] ]
         | no_step; tac; simpl in *; eauto ]
   end.
-
+*)
 Inductive lab_approx : list lab -> env (option I.block) -> list IL.I.block -> Prop :=
   Lai symb L L'
-    (LEQ: forall f f' s Z Lb, 
-             L (counted f) = Some (I.blockI Lb (f',Z,s)) 
-             -> exists i s',   
+    (LEQ: forall f f' s Z Lb,
+             L (counted f) = Some (I.blockI Lb (f',Z,s))
+             -> exists i s',
                  get L' i (IL.I.blockI Z s')
                  /\ labIndices s (drop i symb) = Success s'
                  /\ pos symb f 0 = Some i                                                             /\ lab_approx (drop (S i) symb) (Lb (* [counted f <- Some (I.blockI Lb (f, Z, s))] *)) (drop (S i) L')
                  /\ (forall l b, Lb (counted l) = Some b -> fst (fst (I.block_F b)) = l)
-                 /\ (forall f i' k, pos (drop (S i) symb) f k = Some i' -> Lb (counted f) <> None) 
-                 /\ f = f') 
+                 /\ (forall f i' k, pos (drop (S i) symb) f k = Some i' -> Lb (counted f) <> None)
+                 /\ f = f')
   : lab_approx symb L L'.
 
 Inductive labIndicesSim : I.state -> IL.I.state -> Prop :=
@@ -227,7 +251,7 @@ Inductive labIndicesSim : I.state -> IL.I.state -> Prop :=
     (LL:forall l b, L (counted l) = Some b -> fst (fst (I.block_F b)) = l)
     (EX:forall f i k, pos symb f k = Some i -> L (counted f) <> None)
   : labIndicesSim (L, E, s) (L', E, s').
-      
+
 Lemma pos_add k' symb (f:lab) k i
 : pos symb f k = Some i -> pos symb f (k' + k) = Some (k' + i).
 Proof.
@@ -243,7 +267,7 @@ Proof.
   general induction symb; eauto.
   unfold pos in *; fold pos in *.
   destruct if. f_equal. inv H. omega.
-  orewrite (S (k' + k) = k' + S k) in H. 
+  orewrite (S (k' + k) = k' + S k) in H.
   eauto.
 Qed.
 
@@ -260,11 +284,11 @@ Lemma pos_drop_eq symb (l:lab) x
 : pos symb l 0 = Some x
           -> drop x symb = l::tl (drop x symb).
 Proof.
-  general induction symb. 
+  general induction symb.
   unfold pos in H; fold pos in H. destruct if in H.
   inv H; inv e; eauto.
   destruct x. exfalso. exploit pos_ge; eauto. omega.
-  simpl. erewrite IHsymb; eauto. 
+  simpl. erewrite IHsymb; eauto.
   eapply (pos_sub 1); eauto.
 Qed.
 
@@ -275,21 +299,21 @@ Proof.
   general induction n; simpl; eauto.
   destruct symb; simpl.
   + inv H.
-  + eapply IHn; eauto. simpl in H; destruct if in H. 
-    * inv H. 
+  + eapply IHn; eauto. simpl in H; destruct if in H.
+    * inv H.
     * eapply (pos_sub 1); eauto.
 Qed.
 
 Lemma labIndicesSim_sim σ1 σ2
-  : labIndicesSim σ1 σ2 -> sim σ1 σ2.
+  : labIndicesSim σ1 σ2 -> bisim σ1 σ2.
 Proof.
   revert σ1 σ2. cofix; intros.
   destruct H; destruct s; simpl in *; try monadS_inv EQ.
-  - case_eq (exp_eval E e); intros. 
+  - case_eq (exp_eval E e); intros.
     + one_step. eapply labIndicesSim_sim; econstructor; eauto.
     + no_step.
   - case_eq (exp_eval E e); intros.
-    case_eq (val2bool v); intros; one_step; eapply labIndicesSim_sim; econstructor; eauto. 
+    case_eq (val2bool v); intros; one_step; eapply labIndicesSim_sim; econstructor; eauto.
     no_step.
   - case_eq (L (counted l)); intros.
     + destruct b as [? [[l0 Z'] s']].
@@ -304,41 +328,49 @@ Proof.
       econstructor; eauto. subst l0.
       * simpl.
         econstructor. simpl; intros; dcr.
-        lud. inv H7.         
+        lud. inv H7.
         assert (f = f') by (destruct f, f'; simpl in *; congruence); subst.
         do 2 eexists. split.
         eapply drop_get with (n:=0). orewrite (x + 0 = x). eauto.
-        intuition. 
+        intuition.
         eapply pos_plus. orewrite (x + 0 = x); eauto.
         simpl in *. repeat rewrite drop_tl. auto.
         eapply H6. simpl in H9. rewrite drop_tl in H9. eapply H9. eauto.
         inv H4.
         edestruct (LEQ0); eauto. destruct H10; dcr.
-        eexists (S x0), x2. split; eauto using get. 
+        eexists (S x0), x2. split; eauto using get.
         eapply drop_get. orewrite (x + S x0 = S x + x0). eapply get_drop. eauto.
         repeat rewrite drop_tl in *. repeat rewrite drop_drop in *.
         orewrite (S x0 + x = x0 + S x); eauto.
-        repeat (split; eauto). 
+        repeat (split; eauto).
         exploit pos_drop_eq; [eapply H2|].
         rewrite X. unfold pos; fold pos. destruct if. congruence.
         rewrite drop_tl. eapply (pos_add 1); eauto.
       * subst l0. intros. lud. inv H7.
         assert (l = l0) by (destruct l, l0; simpl in *; congruence); subst.                 simpl; eauto.
         eapply H5; eauto.
-      * subst l. intros. lud. congruence. eapply H6; eauto. 
-        exploit pos_drop_eq; [eapply H2|]. 
+      * subst l. intros. lud. congruence. eapply H6; eauto.
+        exploit pos_drop_eq; [eapply H2|].
         rewrite X in H7. unfold pos in H7; fold pos in H7.
         destruct if in H7. destruct f, l0; simpl in *; congruence.
         simpl. rewrite <- drop_tl. eauto.
-      * subst l. no_step. 
+      * subst l. no_step.
       * subst. no_step.
         edestruct LEQ as [? [? ?]]; eauto; dcr.
         get_functional; subst; simpl in *. congruence.
     + eapply option2status_inv in EQ0. exfalso. eapply EX; eauto.
   - no_step.
+  - case_eq (omap (exp_eval E) Y); intros.
+    + extern_step.
+      * eexists (ExternI f l 0); eexists; try (now (econstructor; eauto)).
+      * eexists; split. econstructor; eauto.
+        eapply labIndicesSim_sim; econstructor; eauto.
+      * eexists; split. econstructor; eauto.
+        eapply labIndicesSim_sim; econstructor; eauto.
+    + no_step.
   - one_step. eapply labIndicesSim_sim. econstructor; eauto.
-    econstructor. intros. 
-    + lud. 
+    econstructor. intros.
+    + lud.
       * inv H. do 2 eexists.
         split. econstructor. intuition. unfold pos; fold pos.
         destruct if; eauto. cbv in n; destruct f, f'; simpl in *; congruence.
@@ -348,17 +380,16 @@ Proof.
         split; eauto. split; eauto.
         unfold pos; fold pos. destruct if; eauto.
                                          congruence.
-        intros. eapply (pos_add 1); eauto. 
-    + intros. lud; eauto. 
+        intros. eapply (pos_add 1); eauto.
+    + intros. lud; eauto.
       inv H; eauto. destruct l, l0; simpl in *; congruence; eauto.
-    + intros. lud. congruence. 
-      unfold pos in H; fold pos in H. 
+    + intros. lud. congruence.
+      unfold pos in H; fold pos in H.
       destruct if in H. congruence. eapply EX; eauto.
 Qed.
 
-(* 
+(*
 *** Local Variables: ***
 *** coq-load-path: (("../" "Lvc")) ***
 *** End: ***
 *)
-
